cogent/llvm/checker/coq/Main.v
@@ -6,58 +6,22 @@ From Vellvm Require Import LLVMAst.
 From Checker Require Import Cogent Compiler Denote.
 From Input Require Import LLVM Source.
 
-(* Definition checkExp (cogentExp : expr) (llvmExp : exp typ) : Prop := compile cogentExp = llvmExp. *)
-
 Import ListNotations.
 
-(* Compute run prog. *)
+(* Semantics *)
 
-(* Open Scope cogent_scope.
-Definition prog : expr := `1 `+ `2 `* `3.
-Compute (burn 100 (denote_expr prog)). *)
+Compute burn 50 (run_cogent CogentInput "main" UUnit).
 
-(* LLVM Import *)
-
-(* Check LLVMInput. *)
-
-(* Definition never : block typ := mk_block (Name "never") [] [] (IVoid 0%Z, TERM_Ret_void) None. *)
-
-(* Definition fixer : list (toplevel_entity typ (list (block typ))) -> list (toplevel_entity typ (block typ * list (block typ))) :=
-  map (fun tle =>
-    match tle with
-      | TLE_Definition d =>
-          let i := df_instrs d in
-            TLE_Definition (mk_definition _ (df_prototype d) (df_args d) (hd never i, tl i))
-      | TLE_Comment x =>  TLE_Comment x
-      | TLE_Target x => TLE_Target x
-      | TLE_Datalayout x => TLE_Datalayout x
-      | TLE_Declaration x => TLE_Declaration x
-      | TLE_Type_decl x y => TLE_Type_decl x y
-      | TLE_Source_filename x => TLE_Source_filename x
-      | TLE_Global x => TLE_Global x
-      | TLE_Metadata x y => TLE_Metadata x y
-      | TLE_Attribute_group x y => TLE_Attribute_group x y
-    end
-  ). *)
-
-(* Definition mcfg := mcfg_of_tle (fixer LLVMInput). *)
-
-(* Definition funs := m_definitions mcfg. *)
-
-(* Import D. *)
-
-(* Compute function_denotation. *)
-
-(* Definition bodies := map df_instrs funs. *)
-
-(* Check map denote_cfg bodies. *)
-
-(* Definition main_args := [UVALUE_I64 (DynamicValues.Int64.zero); UVALUE_Addr (Addr.null)]. *)
-
-(* Compute  (burn 1000 (denote_vellvm_main (mcfg_of_tle LLVMInput))). *)
-
-(* Cogent Import *)
+(* Compile to AST *)
 
 Compute compile_cogent CogentInput.
 
-Compute burn 50 (run_cogent CogentInput "main" UUnit).
+(* Compile to string *)
+
+From QuickChick Require Import QuickChick.
+From Vellvm Require Import ShowAST.
+
+Local Open Scope string.
+
+Compute match (compile_cogent CogentInput) with inl m => m | inr tles => newline ++ (show tles) end.
+
